src/tls/HSL.Receive.fsti
@@ -17,54 +17,8 @@ module HSM = Parsers.Handshake
 module HSM12 = Parsers.Handshake12
 module HSM13 = Parsers.Handshake13
 
-#reset-options
-   "--max_fuel 0 --max_ifuel 0 \
-    --using_facts_from '* -FStar.Tactics -FStar.Reflection -FStar.UInt128 -FStar.Math -LowParse +LowParse.Low.Base +LowParse.Spec.Base'"
+#reset-options "--max_fuel 0 --max_ifuel 0 --using_facts_from '* -FStar.Tactics -FStar.Reflection'"
 
-
-    // --using_facts_from 'Prims FStar LowStar -FStar.Reflection -FStar.Tactics -FStar.UInt128 -FStar.Math' \
-    // --using_facts_from 'Mem HSL Types_s Words_s Spec.Hash.Definitions.bytes' \
-    // --using_facts_from 'TLSError'"
-
-
-// /// HandshakeMessages related definitions
-
-// type msg = HSM.hs_msg
-
-// /// Specifies which messages indicate the end of incoming flights
-// /// Triggers their Handshake processing
-
-// let end_of_flight : msg -> bool =
-//   let open HandshakeMessages in
-//   function
-//   | ClientHello _
-//   | HelloRetryRequest _
-//   | EndOfEarlyData
-//   | ServerHello _
-//   | ServerHelloDone
-//   | NewSessionTicket13 _
-//   | Finished _ -> true
-//   | _ -> false
-// // No support for binders yet -- comment copied from HandshakeLog
-
-
-// /// Specifies which messages require an intermediate transcript hash
-// /// in incoming flights. In doubt, we hash!
-
-// let tagged : msg -> bool =
-//   let open HSM in
-//   function
-//   | ClientHello _
-//   | ServerHello _
-//   | EndOfEarlyData        // for Client finished -- comment (and other comments below) copied from HandshakeLog
-//   | Certificate13 _       // for CertVerify payload in TLS 1.3
-//   | EncryptedExtensions _ // For PSK handshake: [EE; Finished]
-//   | CertificateVerify _   // for ServerFinish payload in TLS 1.3
-//   | ClientKeyExchange _   // only for client signing
-//   | NewSessionTicket _    // for server finished in TLS 1.2
-//   | Finished _ -> true     // for 2nd Finished
-//   | _ -> false
-// // NB CCS is not explicitly handled here, but can trigger tagging and end-of-flights -- comment copied from HandshakeLog
 
 /// HSL main API
 
@@ -90,9 +44,9 @@ val region_of : hsl_state -> GTot Mem.rgn
 
 val index_from_to : st:hsl_state -> HS.mem -> GTot (option range_t)
 
-/// Bytes parsed so far
+/// Bytes parsed so far, in the current flight
 
-val parsed_bytes : st:hsl_state -> HS.mem -> GTot hbytes
+val parsed_bytes : st:hsl_state -> HS.mem -> GTot bytes
 
 /// The invariant is quite light, includes liveness of local state etc.
 
@@ -118,11 +72,8 @@ val frame_hsl_state (st:hsl_state) (h0 h1:HS.mem) (l:B.loc)
       invariant st h1)
 
 
-/// AR: 01/29: verifying this create_post takes a long time, TODO: profile
-
 /// Creation of the log
 unfold
-private
 let create_post (r:Mem.rgn)
   : HS.mem -> hsl_state -> HS.mem -> Type0
   = fun h0 st h1 ->
@@ -148,8 +99,6 @@ val create (r:Mem.rgn)
 
 type b8 = B.buffer uint_8
 
-module HSM13 = Parsers.Handshake13
-
 module EE  = Parsers.Handshake13_m_encrypted_extensions
 module Fin = Parsers.Handshake13_m_finished
 
@@ -164,15 +113,16 @@ type flight_ee_fin = {
 let valid_flight_t 'a =
   (flt:'a) -> (flight_end:uint_32) -> (b:b8) -> (h:HS.mem) -> Type0
 
-
-/// AR: 01/29: up to this point proofs are fine, but beyond this the performance drops
-
-let valid_parsing (msg:HSM13.handshake13) (from to:uint_32) (buf:b8{from <= to /\ B.len buf == to - from}) (h:HS.mem) =
-  let parser = HSM13.handshake13_parser in
-  let slice = { LP.base = buf; LP.len = to - from } in
-  LP.valid parser h slice from /\
-  LP.contents parser h slice from == msg /\
-  LP.content_length parser h slice from == UInt32.v (to - from)
+let valid_parsing13
+  (msg:HSM13.handshake13)
+  (from to:uint_32)
+  (buf:b8{from <= to /\ B.len buf == to - from})
+  (h:HS.mem)
+  = let parser = HSM13.handshake13_parser in
+    let slice = { LP.base = buf; LP.len = to - from } in
+    LP.valid parser h slice from /\
+    LP.contents parser h slice from == msg /\
+    LP.content_length parser h slice from == UInt32.v (to - from)
 
 let valid_flight_ee_fin : valid_flight_t flight_ee_fin =
   fun (flt:flight_ee_fin) (flight_end:uint_32) (b:b8) (h:HS.mem) ->
@@ -184,8 +134,8 @@ let valid_flight_ee_fin : valid_flight_t flight_ee_fin =
   (let ee_buf = B.gsub b flt.begin_ee (flt.begin_fin - flt.begin_ee) in
    let fin_buf = B.gsub b flt.begin_fin (flight_end - flt.begin_fin) in
    
-   valid_parsing (HSM13.M_encrypted_extensions (G.reveal flt.ee_msg)) flt.begin_ee flt.begin_fin ee_buf h /\
-   valid_parsing (HSM13.M_finished (G.reveal flt.fin_msg)) flt.begin_fin flight_end fin_buf h)
+   valid_parsing13 (HSM13.M_encrypted_extensions (G.reveal flt.ee_msg)) flt.begin_ee flt.begin_fin ee_buf h /\
+   valid_parsing13 (HSM13.M_finished (G.reveal flt.fin_msg)) flt.begin_fin flight_end fin_buf h)
 
 let range_extension (r0:option range_t) (from to:uint_32) =
     from <= to /\
@@ -220,30 +170,30 @@ let update_window (r0:option range_t)
 
 unfold private
 let receive_post 
-      (st:hsl_state)
-      (b:b8)
-      (from to:uint_32)
-      (f:valid_flight_t 'a)
-      (h0:HS.mem)
-      (x:TLSError.result (option 'a))
-      (h1:HS.mem) =
-  basic_pre_post st b from to h0 /\
-  B.modifies (footprint st) h0 h1 /\  //only local footprint is modified
-  (let open FStar.Error in
-   match x, index_from_to st h1 with
-   | Error _, _ -> True  //underspecified
-   | Correct None, Some r ->  //waiting for more data
-     let start = fst r in
-     let finish = snd r in
-     finish == to /\
-     parsed_bytes st h1 == B.as_seq h0 (B.gsub b start (finish - start)) /\
-     index_from_to st h1 == update_window (index_from_to st h0) from to
-   | Correct (Some flt), None ->
-     f flt to b h1 /\  //flight specific postcondition
-     //Internal state for partial parse is reset
-     //Ready to receive another flight
-     parsed_bytes st h1 == Seq.empty
-   | _ -> False)
+  (st:hsl_state)
+  (b:b8)
+  (from to:uint_32)
+  (f:valid_flight_t 'a)
+  (h0:HS.mem)
+  (x:TLSError.result (option 'a))
+  (h1:HS.mem)
+  = basic_pre_post st b from to h0 /\
+    B.modifies (footprint st) h0 h1 /\  //only local footprint is modified
+    (let open FStar.Error in
+     match x, index_from_to st h1 with
+     | Error _, _ -> True  //underspecified
+     | Correct None, Some r ->  //waiting for more data
+       let start = fst r in
+       let finish = snd r in
+       finish == to /\
+       parsed_bytes st h1 == B.as_seq h0 (B.gsub b start (finish - start)) /\
+       index_from_to st h1 == update_window (index_from_to st h0) from to
+     | Correct (Some flt), None ->
+       f flt to b h1 /\  //flight specific postcondition
+       //Internal state for partial parse is reset
+       //Ready to receive another flight
+       parsed_bytes st h1 == Seq.empty
+     | _ -> False)
 #pop-options
 
 val receive_flight_ee_fin (st:hsl_state) (b:b8) (from to:uint_32)
@@ -251,307 +201,3 @@ val receive_flight_ee_fin (st:hsl_state) (b:b8) (from to:uint_32)
        (requires basic_pre_post st b  from to)
        (ensures  receive_post st b from to valid_flight_ee_fin)
 
-// val receive_flight_c_ske_shd (st:hsl_state) (b:b8) (from to:uint_32)
-//   : ST (TLSError.result (option flight_c_ske_shd))
-//        (requires basic_pre_post st b from to)
-//        (ensures  receive_post st b from to valid_flight_c_ske_shd)
-
-
-(*
- * framing for local footprints, and input index etc. since they are stateful
- * output index may be we don't need (no incremental serializations)
- * do we need the writing bit, it was inconclusive the other day
- * reset of HSL state?
- * currently we are not telling the client that parsing of the input buffer for current flight started at the end index of last flight, may be that's ok?
- *)
-
-
-// unfold private let receive_post (st:hsl_state) (p:uint_32)
-//   : HS.mem -> (TLSError.result (option (
-//                                flight_t &
-//                                G.erased (list msg) &
-//                                uint_32 & uint_32))) -> HS.mem -> Type0
-//   = fun h0 r h1 ->  
-//     let open FStar.Error in
-//     let oa = hash_alg h0 st in
-//     let t0 = transcript h0 st in
-//     let t1 = transcript h1 st in
-//     (match r with
-//      | Error _ -> True  //underspecified
-//      | Correct None -> t0 == t1  //waiting for more data
-//      | Correct (Some (flt, ms, p0, p1, hs)) ->
-//        let ms = G.reveal ms in
-//        t1 == t0 @ ms /\  //added ms to the transcript
-//        writing h1 st /\  //Handshake can now write
-//        p <= hsl_input_buf_len st /\
-//        p0 <= p1 /\ p1 <= p /\  //returned indices are valid in the input buffer
-//        msg_list_parsing_of ms st p0 p1 h1 /\  //ms is a valid parsing of input buffer contents between p0 and p1
-//        flight_parsing_of flt ms st h1 /\  //the indices in the returned flight are valid parsings
-//        (match oa with
-//         | Some a -> tags a t0 ms hs  //hashed properly
-//         | None -> hs == []))
-
-
-
-
-
-(*
- * CF: make these fine grained, in collaboration with HS
- *)
-// type flight_t =
-//   | F_HRR: init:uint_32 -> len:uint_32 -> flight_t
-//   | F_SH: init:uint_32 -> len:uint_32 -> flight_t
-//   | F_C_SKE_SHD: c_init:uint_32 -> c_len:uint_32 ->
-//                  ske_init:uint_32 -> ske_len:uint_32 -> 
-// 		 -> erased certificate -> erased ske ->
-// 		 flight_t
-//   | F_C_SKE_CR_SHD: c_init:uint_32 -> c_len:uint_32 ->
-//                     ske_init:uint_32 -> ske_len:uint_32 ->
-//                     cr_init:uint_32 -> cr_len:uint_32 -> flight_t
-//   | F_EE_C13_CV_Fin: ee_init:uint_32 ->
-//                      c13_init:uint_32 ->
-// 		     cv_init:uint_32 ->
-// 		     fin_init:uint_32 -> fin_len:uint_32 -> flight_t
-//   | F_EE_CR13_C13_CV_Fin: ee_init:uint_32 -> ee_len:uint_32 ->
-//                           cr13_init:uint_32 -> cr13_len:uint_32 ->
-// 			  c13_init:uint_32 -> c13_len:uint_32 ->
-// 			  cv_init:uint_32 -> cv_len:uint_32 ->
-// 			  fin_init:uint_32 -> fin_len:uint_32 -> flight_t
-//   | F_EE_Fin: ee_init:uint_32 -> ee_len:uint_32 ->
-//               fin_init:uint_32 -> fin_len:uint_32 -> flight_t
-//   | F_Fin: fin_init:uint_32 -> fin_len:uint_32 -> flight_t
-//   | F_CH: ch_init:uint_32 -> ch_len:uint_32 -> flight_t
-//   | F_CH_Bind: ch_init:uint_32 -> ch_len:uint_32 ->
-//                bind_init:uint_32 -> bind_len:uint_32 -> flight_t
-//   | F_C13_CV_Fin: c13_init:uint_32 -> c13_len:uint_32 ->
-//                   cv_init:uint_32 -> cv_len:uint_32 ->
-// 		  fin_init:uint_32 -> fin_len:uint_32 -> flight_t
-//   | F_EoED: flight_t
-//   | F_NST13: nst13_init:uint_32 -> nst13_len:uint_32 -> flight_t
-
-
-// /// Current flight that has been dispatched to Handshake but is in the process of being hashed
-
-// val current_flight (st:hsl_state) (h:HS.mem) : GTot flight_t
-
-
-// type flgithval current_hash_index (st:hsl_state) (h:HS.mem) : GTot uint_32
-
-// /// Framing of current flight, current flight index w.r.t. modifications to local state
-
-
-// let is_valid_hash_index (st:hsl_state) (i:uint_32) (h:HS.mem) : GTot bool =
-//   let flt = current_flight st h in
-//   match flt with
-//   | F_HRR init len -> i == init + len
-//   | _ -> admit ()
-
-// let end_of_flight_index (st:hsl_state) (h:HS.memt) : GTot uint_32 =
-//   let flt = current_flight st h in
-//   match flt with
-//   | F_HRR init len -> init + len
-//   | _ -> admit ()
-
-
-// /// Do we need to provide 
-
-// (*
-//  * Separate into two: one that computes hash and one that returns it
-//  * Transcript should reflect partial flights that have been hashed
-//  * Additional state in HSL to maintain this
-//  *)
-// val hash (st:hsl_state) (i:uint_32)
-//   : ST unit (requires (fun h0 -> is_valid_hash_index st i /\ i > current_hash_index st h))
-//             (ensures  (fun h0 _ h1 -> current_hash_index st h1 == i /\ modifies (hsl_local_footprint st) h0 h1 /\
-// 	               i == end_of_flight_index st h0 ==>
-// 		         (writing h1 st /\
-// 			  transcript h1 st == transcript h0 st @ current_hs_flight st h0)))
-
-
-
-// // Option a.
-
-// // HSL doesn't care what you hash on the receive side.
-// // HS maintains enough invariants to make sure
-// // it has hashed the input messages using the ghost messages HSL.receive returned.
-// // HS maintains the postcondition that transcript has increased when it calls HSL.hash
-// // Generic precondition of calling HSL.hash
-
-// // Pros: helps with binders, can hash in the middle of messages
-
-// // Cons: writing capability maintenance moves to HS for the input flight hashing part, except when HSL is in the middle of reading a flight, HSL switches to writing when it has received a flight
-
-// // hash (i:uint_32) (j:uint_32)
-// //      (msgs:erased (list msgs){msgs is parsing of input buffer from i to j})
-// //      (* can we make it so that it is not erased (list (erased msg)) *)
-// //   : ensures (transcript is appended to by msgs)
-
-
-// // On the writing side, it is the same--hashing is done by HSL when HS calls HSL.send
-
-// // send (...)
-// //   : ensures (transcript is extedned automatically)
-
-
-// // -- State of hash
-// // -- State of incoming flight, what we are trying to receive
-// // -- Internal state of HSL is like a tree what all flights can we receive
-// // -- Precondition of receive depending on the states
-// //    Next kind of flight? Should HSL keep track of it?
-// // -- No flight_t and having ad-hoc receive messages
-
-
-// // Whatever we send is a valid receive flight at the other end?
-// // Peer state machine will accept what we send
-
-// #reset-options "--max_fuel 0 --initial_ifuel 1 --max_ifuel 1"
-
-// /// TODO: should come from QD
-
-
-// val hrr_parser : parser_t HSM.hrr
-// val sh_parser : parser_t HSM.sh
-// val c_parser : parser_t HSM.crt
-// val ske_parser : parser_t HSM.ske
-// val cr_parser : parser_t HSM.cr
-
-// unfold let valid_parsing (#a:Type) (m:a) (parser:parser_t a) (buf:B.buffer uint_8) (h:HS.mem) =
-//   match LP.parse parser (B.as_seq h buf) with
-//   | None -> False
-//   | Some (parse, consumed) -> parse == m /\ consumed == B.length buf
-
-// unfold let valid_init_and_len (init len:uint_32) (st:hsl_state) =
-//   init <= len /\ within_bounds (Unsigned W32) (v init + v len) /\ init + len <= hsl_input_buf_len st  
-
-// /// Predicate for flight being a valid parsing
-// /// In addition to this, the postcondition of receive also establishes valid parsing of the transcript itself
-
-// let flight_parsing_of (flt:flight_t) (msgs:hs_transcript) (st:hsl_state) (h:HS.mem) =
-//   match flt with
-//   | F_HRR init len ->
-//     valid_init_and_len init len st /\
-//     (match msgs with
-//      | [ HSM.HelloRetryRequest r ] -> valid_parsing r hrr_parser (B.gsub (hsl_input_buf st) init len) h
-//      | _ -> False)
-
-//   | F_SH init len ->
-//     valid_init_and_len init len st /\
-//     (match msgs with
-//      | [ HSM.ServerHello sh ] -> valid_parsing sh sh_parser (B.gsub (hsl_input_buf st) init len) h
-//      | _ -> False)
-
-//   | F_C_SKE_SHD c_init ske_init ske_len ->
-//     valid_init_and_len c_init c_len st /\ valid_init_and_len ske_init ske_len st /\
-//     (match msgs with
-//      | [ HSM.Certificate c; HSM.ServerKeyExchange ske; HSM.ServerHelloDone ] ->
-//        valid_parsing c c_parser (B.gsub (hsl_input_buf st) c_init c_len) h /\
-//        valid_parsing ske ske_parser (B.gsub (hsl_input_buf st) ske_init ske_len) h
-//      | _ -> False)
-
-//   | F_C_SKE_CR_SHD c_init c_len ske_init ske_len cr_init cr_len ->
-//     valid_init_and_len c_init c_len st /\ valid_init_and_len ske_init ske_len st /\ valid_init_and_len cr_init cr_len st /\
-//     (match msgs with
-//      | [ HSM.Certificate c; HSM.ServerKeyExchange ske; HSM.CertificateRequest cr; HSM.ServerHelloDone ] ->
-//        valid_parsing c c_parser (B.gsub (hsl_input_buf st) c_init c_len) h /\
-//        valid_parsing ske ske_parser (B.gsub (hsl_input_buf st) ske_init ske_len) h /\
-//        valid_parsing cr cr_parser (B.gsub (hsl_input_buf st) cr_init cr_len) h
-//      | _ -> False)
-
-//   //TODO: fill other entries similarly
-
-//   | _ -> False
-       
-  
-// /// TODO: Should come from QD
-
-// val hs_transcript_parser : LP.parser (LP.strong_parser_kind 8 8 ({ LP.parser_kind_metadata_total = true })) hs_transcript
-
-// (* msgs is parsing of the input sub-buffer between p0 and p1 *)
-// unfold private let msg_list_parsing_of (msgs:hs_transcript) (st:hsl_state)
-//                                        (p0:uint_32) (p1:uint_32{p0 <= p1 /\ p1 <= hsl_input_buf_len st})
-// 			               (h:HS.mem)
-//   = let delta = p1 - p0 in
-//     let sub = B.gsub (hsl_input_buf st) p0 delta in
-//     match LP.parse hs_transcript_parser (B.as_seq h sub) with
-//     | None -> False
-//     | Some (parse, consumed) -> parse == msgs /\ consumed == v delta
-
-// (*
-//  * CF: Remember indices in the input buffer for transcripts
-//  *     May be just keep index until t0
-//  *     For incremental hashing for t1, keep states in between
-//  *     Hashing can be part of the state
-//  *     After delivering the flight, and before starting new flight,
-//  *       remember where is hashing state (index)
-//  *     Also hashing state is just Evercrypt hash state
-//  *     Return hash value on the caller stack
-//  *     Transcript is the hashed transcript? Add messages to transcrip
-//  *       when hashed after call to HS
-//  *     HSLog maintains hashed transcript
-//  *       and indices for the last flight returned -- so that it can relate Hash calls from HS
-//  *)
-
-// (* pair of ints can be computed from flight_t *)
-// (* flight_t with indices and erased messages with postconditions for relating them *)
-
-
-// //TODO: delay the hashing OR Handshake explicitly calls Log to compute the digest 
-
-
-// /// TODO: receive_CCS
-
-
-// /// Send API
-
-// /// TODO: should come from QD
-
-// val msg_parser : parser_t msg
-
-// unfold private let msg_parsing_of (m:msg) (st:hsl_state)
-//                                   (p0:uint_32) (p1:uint_32{p0 <= p1 /\ p1 <= hsl_output_buf_len st})
-// 			          (h:HS.mem)
-//   = let delta = p1 - p0 in
-//     let sub = B.gsub (hsl_output_buf st) p0 delta in
-//     match LP.parse msg_parser (B.as_seq h sub) with
-//     | None -> False
-//     | Some (parse, consumed) -> parse == m /\ consumed == v delta
-
-// unfold private let send_pre (st:hsl_state) (p:uint_32) (m:G.erased msg)
-//   : HS.mem -> Type0
-//   = fun h0 ->
-//     let open HandshakeMessages in
-//     hsl_invariant h0 st /\  //invariant holds
-//     hsl_output_index h0 st <= p /\ p <= hsl_output_buf_len st /\  //p is in range of output buffer
-//     msg_parsing_of (G.reveal m) st (hsl_output_index h0 st) p h0 /\  //m is a valid parsing of sub-buffer between p0 and p1
-//     writing h0 st /\  //Handshake is allowed to write
-//     valid_transcript (transcript h0 st @ [G.reveal m]) /\  //valid transcript
-//     (match G.reveal m with  //copied from HandshakeLog as is
-//      | HelloRetryRequest req -> Some? (C.cipherSuite_of_name req.hrr_cipher_suite)
-//      | _ -> True)
-
-// unfold private let send_post (st:hsl_state) (p:uint_32) (m:G.erased msg)
-//   : HS.mem -> unit -> HS.mem -> Type0
-//   = fun h0 _ h1 ->
-//     B.modifies (hsl_local_footprint st) h0 h1 /\  //only local footprint is modified
-//     writing h1 st /\  //writing capability remains
-//     hash_alg h1 st == hash_alg h0 st /\  //hash algorithm is same as before
-//     transcript h1 st == transcript h0 st @ [G.reveal m] /\  //transcript includes m
-//     hsl_invariant h1 st /\  //invariant hold
-//     hsl_input_index h1 st == hsl_input_index h0 st /\  //input buffer index remains same
-//     hsl_output_index h1 st == p  //output buffer index is advanced to p
-
-// val send (st:hsl_state) (p:uint_32) (m:G.erased msg)
-//   : ST unit (requires (send_pre st p m))
-//             (ensures  (send_post st p m))
-		       
-// /// hash_tag API
-
-// /// TODO: the postcondition fails to typecheck
-
-// #push-options "--admit_smt_queries true"
-// val hash_tag (a:Hash.alg) (st:hsl_state)
-//   : ST (Hash.tag a) (requires (fun h0 -> hsl_invariant h0 st))
-//                     (ensures  (fun h0 r h1 ->
-// 		               let bs = transcript_bytes (transcript h1 st) in
-// 			       h0 == h1 /\ Hashing.CRF.hashed a bs /\ r == Hash.h a bs))
-// #pop-options
